some tests worked

theories/L2_typeStripped/test_wcbvEval.v
@@ -12,6 +12,37 @@ Local Open Scope bool.
 Local Open Scope list.
 Set Implicit Arguments.
 
+
+(** vector addition **)
+Require Coq.Vectors.Vector.
+Print Fin.t.
+Print Vector.t.
+
+Definition vplus (n:nat) :
+  Vector.t nat n -> Vector.t nat n -> Vector.t nat n := (Vector.map2 plus).
+Definition v01 : Vector.t nat 2 :=
+  (Vector.cons nat 0 1 (Vector.cons nat 1 0 (Vector.nil nat))).
+Definition v23 : Vector.t nat 2 :=
+  (Vector.cons nat 2 1 (Vector.cons nat 3 0 (Vector.nil nat))).
+Definition vplus0123 := (vplus v01 v23).
+Quote Recursively Definition cbv_vplus0123 := (* [program] of Coq's answer *)
+  ltac:(let t:=(eval cbv in (vplus0123)) in exact t).
+Print cbv_vplus0123.
+(* [Term] of Coq's answer *)
+Definition ans_vplus0123 := Eval cbv in (main (program_Program cbv_vplus0123)).
+(* [program] of the program *)
+Quote Recursively Definition p_vplus0123 := vplus0123.
+Print p_vplus0123.
+Definition P_vplus0123 := Eval cbv in (program_Program p_vplus0123).
+Print P_vplus0123.
+Goal
+  let env := (env P_vplus0123) in
+  let main := (main P_vplus0123) in
+  wcbvEval (env) 100 (main) = Ret ans_vplus0123.
+  vm_compute. reflexivity.
+Qed.
+
+
 (** a tool for testing **)
 Definition exc_wcbvEval (tmr:nat) (pgm:program): Term :=
   let pgm := L2.compile.program_Program pgm in
